Update Schulze_inv.v

src/Schulze_inv.v
@@ -66,16 +66,16 @@ Section Schulze.
 
   Definition ballot := cand -> nat.
 
-  Inductive State: Type :=
-  | partial: (list ballot * list ballot)  -> (cand -> cand -> Z) -> State
-  | winners: (cand -> bool) -> State.
+  Inductive state: Type :=
+  | partial: (list ballot * list ballot)  -> (cand -> cand -> Z) -> state
+  | winners: (cand -> bool) -> state.
 
 
-  Inductive Count (bs : list ballot) : State -> Type :=
+  Inductive Count (bs : list ballot) : state -> Type :=
   | ax us (m : cand -> cand -> Z) : us = bs -> (forall c d, m c d = 0%Z) ->
       Count bs (partial (us, []) m)             (* zero margin      *)
   | cvalid u us m nm inbs : Count bs (partial (u :: us, inbs) m) ->
-      (forall c, (u c > 0)%nat) ->              (* u is valid       *)
+      (forall c, (0 < u c)%nat) ->              (* u is valid       *)
       (forall c d : cand,
         ((u c < u d)%nat -> nm c d = m c d + 1) (* c preferred to d *) /\
         ((u c = u d)%nat -> nm c d = m c d)     (* c, d rank equal  *) /\
@@ -92,7 +92,7 @@ Section Schulze.
       Count bs (winners w).
 
 
-  Theorem count_inv : ∀ (bs : list ballot) (s : State) (e : Count bs s), 
+  Theorem count_inv : ∀ (bs : list ballot) (s : state) (e : Count bs s), 
     match e as e' in Count _ s' return Count _ s' -> Type 
     with 
     | ax _ us m ha hb => fun (b : Count bs (partial (us, []) m)) => 
@@ -108,4 +108,44 @@ Section Schulze.
     destruct e; exact eq_refl.
   Defined.
 
-End Schulze. 
+
+  Definition count_inv_ax_ret_type {bs : list ballot} (s : state) : 
+    Count bs s -> Prop.
+  Proof.
+    refine 
+      match s as s' return Count _ s' -> Prop 
+      with 
+      | partial (us, vx) m => 
+        match vx as vx' return (Count _ (partial (us, vx') m) -> Prop) with 
+        | [] => fun (c : (Count _ (partial (us, []) m))) => 
+          (∃ (ha : us = bs)  (hb : ∀ c d : cand, m c d = 0),  c = ax _ us m ha hb) ∨
+          (∃ u nm ha hb hc, c = cvalid _ u us nm m [] ha hb hc)
+        | _ => fun _ => IDProp
+        end
+      | winners _ => fun _ => IDProp 
+      end.
+  Defined.
+
+
+  Theorem count_inv_ax : ∀ (bs us : list ballot) (m : cand -> cand -> Z) 
+    (e : Count bs (partial (us , []) m)), 
+    (∃ (ha : us = bs)  (hb : ∀ c d : cand, m c d = 0),  e = ax _ us m ha hb) ∨
+    (∃ u nm ha hb hc, e = cvalid _ u us nm m [] ha hb hc).
+  Proof.
+    intros *.
+    refine 
+      match e as e' in Count _ s' return count_inv_ax_ret_type s' e' with
+      | ax _ us m ha hb => _ 
+      | cvalid _ u _ _ nm inbs ha hb hc => _
+      | _ => _
+      end; cbn; try (exact idProp).
+    +
+      left; repeat eexists; 
+      exact eq_refl.
+    +
+      destruct inbs as [| h t]; cbn. 
+      right; repeat eexists.
+      exact idProp.
+  Defined.
+    
+End Schulze.  
